Initial implementation for byzantine_behavior (faulty) replica. (#2384)
* Initial implementation for byzantine_behavior (faulty) replica.

In this implementation we instantiate the faulty replicas at the
creation of our distributed system. Even though the distributed system
is aware who are the faulty nodes, the replicas themselves don't have
access to this knowledge.

* Added constructors check for FaultyReplica in WF.

* Fixed forall parentheses.

* Addition of Byzantine replicas complete.

* Fix steps to correctly indicate type check.

* Loosened the ensures on CountHonestReplicas.

We can have at minimum 2F+1 replicas to ensure safety,
but the honest ones can be up to 3F+1. Added correction
for this in CountHonestReplicas lemma.

docs/sbft-formal-model/distributed_system.s.dfy
@@ -13,6 +13,7 @@ include "replica.i.dfy"
 include "client.i.dfy"
 include "cluster_config.s.dfy"
 include "messages.dfy"
+include "faulty_replica.i.dfy"
 
 // Before we get here, caller must define a type Message that we'll
 // use to instantiate network.s.dfy.
@@ -22,11 +23,17 @@ module DistributedSystem {
   import opened Messages
   import ClusterConfig
   import Replica
+  import FaultyReplica
   import Client
   import Network
 
-  datatype HostConstants = Replica(replicaConstants:Replica.Constants) | Client(clientConstants:Client.Constants)
-  datatype HostVariables = Replica(replicaVariables:Replica.Variables) | Client(clientVariables:Client.Variables)
+  datatype HostConstants = | Replica(replicaConstants:Replica.Constants)
+                           | FaultyReplica(faultyReplicaConstants:FaultyReplica.Constants)
+                           | Client(clientConstants:Client.Constants)
+
+  datatype HostVariables = | Replica(replicaVariables:Replica.Variables)
+                           | FaultyReplica(faultyReplicaVariables:FaultyReplica.Variables)
+                           | Client(clientVariables:Client.Variables)
 
   datatype Constants = Constants(
     hosts:seq<HostConstants>,
@@ -37,8 +44,12 @@ module DistributedSystem {
       && clusterConfig.WF()
       && clusterConfig.ClusterSize() == NumHosts()
       && |hosts| == NumHosts()
-      && (forall id | clusterConfig.IsReplica(id) :: hosts[id] == HostConstants.Replica(Replica.Constants(id, clusterConfig)))
-      && (forall id | clusterConfig.IsClient(id) :: hosts[id] == HostConstants.Client(Client.Constants(id, clusterConfig)))
+      && (forall id | clusterConfig.IsHonestReplica(id) :: && hosts[id] == HostConstants.Replica(Replica.Constants(id, clusterConfig))
+                                                           && hosts[id].replicaConstants.Configure(id, clusterConfig))
+      && (forall id | clusterConfig.IsFaultyReplica(id) :: && hosts[id] == HostConstants.FaultyReplica(FaultyReplica.Constants(id, clusterConfig))
+                                                           && hosts[id].faultyReplicaConstants.Configure(id, clusterConfig))
+      && (forall id | clusterConfig.IsClient(id) :: && hosts[id] == HostConstants.Client(Client.Constants(id, clusterConfig))
+                                                    && hosts[id].clientConstants.Configure(id, clusterConfig))
     }
   }
 
@@ -49,24 +60,25 @@ module DistributedSystem {
     predicate WF(c: Constants) {
       && c.WF()
       && |hosts| == |c.hosts|
-      && (forall id | c.clusterConfig.IsReplica(id) :: hosts[id].Replica? && hosts[id].replicaVariables.WF(c.hosts[id].replicaConstants))
+      && (forall id | c.clusterConfig.IsHonestReplica(id) :: hosts[id].Replica? && hosts[id].replicaVariables.WF(c.hosts[id].replicaConstants))
       && (forall id | c.clusterConfig.IsClient(id) :: hosts[id].Client? && hosts[id].clientVariables.WF(c.hosts[id].clientConstants))
+      && (forall id | c.clusterConfig.IsFaultyReplica(id) :: hosts[id].FaultyReplica?)
     }
   }
 
   predicate IsCommitted(c:Constants, v:Variables, view:nat, seqID:SequenceID) {
     && v.WF(c)
-    && var ReplicasCommitted := set replicaID | && 0 <= replicaID < c.clusterConfig.N()
+    && var ReplicasCommitted := set replicaID | && c.clusterConfig.F() <= replicaID < c.clusterConfig.N()
                                                 && Replica.QuorumOfPrepares(c.hosts[replicaID].replicaConstants,
                                                                             v.hosts[replicaID].replicaVariables,
                                                                             seqID);
     //TODO: Implement check for hasPrePrepare
-    && |ReplicasCommitted| >= c.clusterConfig.ByzantineSafeQuorum()
+    && |ReplicasCommitted| >= c.clusterConfig.AgreementQuorum()
   }
 
   predicate Init(c:Constants, v:Variables) {
     && v.WF(c)
-    && (forall id | && c.clusterConfig.IsReplica(id) 
+    && (forall id | && c.clusterConfig.IsHonestReplica(id) 
                     :: Replica.Init(c.hosts[id].replicaConstants, v.hosts[id].replicaVariables))
     && (forall id | && c.clusterConfig.IsClient(id)
                     :: Client.Init(c.hosts[id].clientConstants, v.hosts[id].clientVariables))
@@ -79,8 +91,16 @@ module DistributedSystem {
   predicate ReplicaStep(c:Constants, v:Variables, v':Variables, step: Step) {
       && v.WF(c)
       && v'.WF(c)
-      && c.clusterConfig.IsReplica(step.id)
+      && c.clusterConfig.IsHonestReplica(step.id)
       && Replica.Next(c.hosts[step.id].replicaConstants, v.hosts[step.id].replicaVariables, v'.hosts[step.id].replicaVariables, step.msgOps)
+  }
+
+  predicate FaultyReplicaStep(c:Constants, v:Variables, v':Variables, step: Step) {
+      && v.WF(c)
+      && v'.WF(c)
+      && c.clusterConfig.IsFaultyReplica(step.id)
+      && assert v.hosts[step.id].FaultyReplica?; true
+      && FaultyReplica.Next(c.hosts[step.id].faultyReplicaConstants, v.hosts[step.id].faultyReplicaVariables, v'.hosts[step.id].faultyReplicaVariables, step.msgOps)
   }
 
   predicate ClientStep(c:Constants, v:Variables, v':Variables, step: Step) {
